@prefix rdf: <http://www.w3.org/1999/02/22-rdf-syntax-ns#> .
@prefix rdfs: <http://www.w3.org/2000/01/rdf-schema#> .
@prefix owl: <http://www.w3.org/2002/07/owl#> .
@prefix xsd: <http://www.w3.org/2001/XMLSchema#> .
@prefix dct: <http://purl.org/dc/terms/> .
@prefix skos: <http://www.w3.org/2004/02/skos/core#> .
@prefix cc: <http://creativecommons.org/ns#> .
@prefix era: <http://data.europa.eu/949/> .
@prefix era-skos: <http://data.europa.eu/949/concepts/> .

@prefix era-subloctype: <http://data.europa.eu/949/concepts/subsidiary-location-types/> .





#################################################################
#
#    Concept Schemes
#
#################################################################




era-subloctype:SubsidiaryLocationTypes a skos:ConceptScheme ; 
    dct:created "2024-09-24"^^xsd:date ;
    dct:modified "2024-12-16"^^xsd:date ;
    cc:license <https://creativecommons.org/licenses/by/4.0/> ;
    rdfs:comment "Controlled SKOS-based vocabularies defined by the European Union Agency for Railways to describe concepts related to the European railway infrastructure and the vehicles authorized to operate over it."@en ;
    rdfs:label "Subsidiary location types"@en ;
    skos:prefLabel "Subsidiary location types"@en ;
    dct:title "Concept scheme grouping subsidiary location types"@en .



#################################################################
#
#    Concept instances
#
#################################################################


## The subsidiary locations here do not take into account the ones marked as 'to be deleted' or existing classes in the ontology


########## Subsidiary Location Types ##########

era-subloctype:00 a skos:Concept;
  skos:inScheme era-subloctype:SubsidiaryLocationTypes; 
  skos:topConceptOf era-subloctype:SubsidiaryLocationTypes ; 
  skos:note "Value collected from TAF/TAP-TSI code lists"@en;
  skos:notation "00"^^xsd:string;
  skos:prefLabel "Not Defined"@en ;
   .


era-subloctype:04 a skos:Concept;
  skos:inScheme era-subloctype:SubsidiaryLocationTypes; 
  skos:topConceptOf era-subloctype:SubsidiaryLocationTypes ; 
  skos:note "Value collected from TAF/TAP -TSI code lists"@en;
  skos:notation "04"^^xsd:string;
  skos:prefLabel "Sorting Code"@en ;
  skos:definition """Destination station of the single wagon forwarding has a code in order to provide shunting
technology."""@en ;
   .


era-subloctype:05 a skos:Concept;
  skos:inScheme era-subloctype:SubsidiaryLocationTypes; 
  skos:topConceptOf era-subloctype:SubsidiaryLocationTypes ; 
  skos:note "Value collected from TAF/TAP -TSI code lists"@en;
  skos:notation "05"^^xsd:string;
  skos:prefLabel "Vehicle Parking Points"@en ;
  skos:definition """Place for parking rail vehicles."""@en ;
   .

era-subloctype:06 a skos:Concept;
  skos:inScheme era-subloctype:SubsidiaryLocationTypes; 
  skos:topConceptOf era-subloctype:SubsidiaryLocationTypes ; 
  skos:note "Value collected from TAF/TAP -TSI code lists"@en;
  skos:notation "06"^^xsd:string;
  skos:prefLabel "Public Loading Places"@en ;
  skos:definition """Public sidings consist of one or more publicly accessible installation of loading tracks, possibly Private sidings consist of one or more installations of rail infrastructure and loading facilities whose access is generally restricted to the owner. They often belong to industrial, commercial,"""@en ;
  skos:scopeNote "Comment: Register purpose only, not to be used in RU communication"@en ;
   .

era-subloctype:07 a skos:Concept;
  skos:inScheme era-subloctype:SubsidiaryLocationTypes; 
  skos:topConceptOf era-subloctype:SubsidiaryLocationTypes ; 
  skos:note "Value collected from TAF/TAP -TSI code lists"@en;
  skos:notation "07"^^xsd:string;
  skos:prefLabel "Private sidings"@en ;
  skos:definition """Private sidings consist of one or more installations of rail infrastructure and loading facilities whose access is generally restricted to the owner. They often belong to industrial, commercial,
military or other types of premises connected to the public rail network. The layout configuration depends on the individual requirements of the respective user. Sometimes
several private sidings are connected to a feeder track, which in turn is connected to the public network (e.g. in ports). (Sub type to Freight
terminal)"""@en ;
  skos:scopeNote "SLC renamed and will serve as register purpose only, not to be used in RU communication"@en ;
   .

era-subloctype:09 a skos:Concept;
  skos:inScheme era-subloctype:SubsidiaryLocationTypes; 
  skos:topConceptOf era-subloctype:SubsidiaryLocationTypes ; 
  skos:note "Value collected from TAF/TAP -TSI code lists"@en;
  skos:notation "09"^^xsd:string;
  skos:prefLabel "Depot"@en ;
  skos:definition "Place for overhaul or maintenance of the rolling stock"@en ;
   .

era-subloctype:25 a skos:Concept;
  skos:inScheme era-subloctype:SubsidiaryLocationTypes; 
  skos:topConceptOf era-subloctype:SubsidiaryLocationTypes ; 
  skos:note "Value collected from TAF/TAP -TSI code lists"@en;
  skos:notation "25"^^xsd:string;
  skos:prefLabel "Underpass"@en ;
  skos:definition "Undercrossing or underground"@en ;
   .

era-subloctype:28 a skos:Concept;
  skos:inScheme era-subloctype:SubsidiaryLocationTypes; 
  skos:topConceptOf era-subloctype:SubsidiaryLocationTypes ; 
  skos:note "Value collected from TAF/TAP -TSI code lists"@en;
  skos:notation "28"^^xsd:string;
  skos:prefLabel "Sign and board"@en ;
  skos:definition "Static equipment to inform the board staff for train traffic and shunting or the passengers in a station"@en ;
   .

era-subloctype:29 a skos:Concept;
  skos:inScheme era-subloctype:SubsidiaryLocationTypes; 
  skos:topConceptOf era-subloctype:SubsidiaryLocationTypes ; 
  skos:note "Value collected from TAF/TAP -TSI code lists"@en;
  skos:notation "29"^^xsd:string;
  skos:prefLabel "Phase break"@en ;
  skos:definition "Border of the power supply systems"@en ;
   .

era-subloctype:36 a skos:Concept;
  skos:inScheme era-subloctype:SubsidiaryLocationTypes; 
  skos:topConceptOf era-subloctype:SubsidiaryLocationTypes ; 
  skos:note "Value collected from TAF/TAP -TSI code lists"@en;
  skos:notation "36"^^xsd:string;
  skos:prefLabel "Freight yard"@en ;
  skos:definition "A production location which can be used as an origin, intermediate or destination station of a freight train"@en ;
  skos:scopeNote "COM (ECN 1.6), Wagon"@en ;
   .

era-subloctype:37 a skos:Concept;
  skos:inScheme era-subloctype:SubsidiaryLocationTypes; 
  skos:topConceptOf era-subloctype:SubsidiaryLocationTypes ; 
  skos:note "Value collected from TAF/TAP -TSI code lists"@en;
  skos:notation "37"^^xsd:string;
  skos:prefLabel "Loading point"@en ;
  skos:definition "A usage of a physical location. Each loading point is assigned to a DIUM station. Loading point is a customer siding (public or private) used in communication with RUs"@en ;
  skos:scopeNote "COM (ECN1.6),"@en ;
   .

era-subloctype:39 a skos:Concept;
  skos:inScheme era-subloctype:SubsidiaryLocationTypes; 
  skos:topConceptOf era-subloctype:SubsidiaryLocationTypes ; 
  skos:note "Value collected from TAF/TAP -TSI code lists"@en;
  skos:notation "39"^^xsd:string;
  skos:prefLabel "Reservation code"@en ;
  skos:definition "Attribute of the location that can be start or end point of traveling with"@en ;
  skos:scopeNote "Specific for Retail"@en ;
   .

era-subloctype:40 a skos:Concept;
  skos:inScheme era-subloctype:SubsidiaryLocationTypes; 
  skos:topConceptOf era-subloctype:SubsidiaryLocationTypes ; 
  skos:note "Value collected from TAF/TAP -TSI code lists"@en;
  skos:notation "40"^^xsd:string;
  skos:prefLabel "Metastation"@en ;
  skos:definition "A location that forms the link between different stations that are"@en ;
  skos:scopeNote "Specific for Retail"@en ;
   .

era-subloctype:41 a skos:Concept;
  skos:inScheme era-subloctype:SubsidiaryLocationTypes; 
  skos:topConceptOf era-subloctype:SubsidiaryLocationTypes ; 
  skos:note "Value collected from TAF/TAP -TSI code lists"@en;
  skos:notation "41"^^xsd:string;
  skos:prefLabel "Company specific Identifier"@en ;
  skos:definition "Similar code as primary location code. used as key to legacy location coding."@en ;
 
   .

era-subloctype:42 a skos:Concept;
  skos:inScheme era-subloctype:SubsidiaryLocationTypes; 
  skos:topConceptOf era-subloctype:SubsidiaryLocationTypes ; 
  skos:note "Value collected from TAF/TAP -TSI code lists"@en;
  skos:notation "42"^^xsd:string;
  skos:prefLabel "DIUM"@en ;
  skos:definition "DIUM stations - Places of acceptance/delivery/handover Commercial Station open into international traffic of goods (tariff point or contract station included in DIUM) â€“ consignment acceptance/delivery station (loading points are excluded and covered by TypeCode 37). Could be a location to handover wagons."@en ;
  skos:scopeNote "COM [ECN 1.6],"@en ;
   .

era-subloctype:43 a skos:Concept;
  skos:inScheme era-subloctype:SubsidiaryLocationTypes; 
  skos:topConceptOf era-subloctype:SubsidiaryLocationTypes ; 
  skos:note "Value collected from TAF/TAP -TSI code lists"@en;
  skos:notation "43"^^xsd:string;
  skos:prefLabel "Passengers cars loading"@en ;
  skos:definition "A place of physical location on the open access network where passengers can load/unload their car"@en ;
  
   .

era-subloctype:45 a skos:Concept;
  skos:inScheme era-subloctype:SubsidiaryLocationTypes; 
  skos:topConceptOf era-subloctype:SubsidiaryLocationTypes ; 
  skos:note "Value collected from TAF/TAP -TSI code lists"@en;
  skos:notation "45"^^xsd:string;
  skos:prefLabel "Sewage dump"@en ;
  skos:definition "A place for cleaning purposes - disposal of the waste."@en ;
  
   .

era-subloctype:46 a skos:Concept;
  skos:inScheme era-subloctype:SubsidiaryLocationTypes; 
  skos:topConceptOf era-subloctype:SubsidiaryLocationTypes ; 
  skos:note "Value collected from TAF/TAP -TSI code lists"@en;
  skos:notation "46"^^xsd:string;
  skos:prefLabel "Refuelling"@en ;
  skos:definition "Location where refuelling takes"@en ;
  
   .

era-subloctype:47 a skos:Concept;
  skos:inScheme era-subloctype:SubsidiaryLocationTypes; 
  skos:topConceptOf era-subloctype:SubsidiaryLocationTypes ; 
  skos:note "Value collected from TAF/TAP -TSI code lists"@en;
  skos:notation "47"^^xsd:string;
  skos:prefLabel "Mains Supply"@en ;
  skos:definition "Location where energy supply can be provided for the rolling stock e.g. preheating."@en ;
  
   .


era-subloctype:48 a skos:Concept;
  skos:inScheme era-subloctype:SubsidiaryLocationTypes; 
  skos:topConceptOf era-subloctype:SubsidiaryLocationTypes ; 
  skos:note "Value collected from TAF/TAP -TSI code lists"@en;
  skos:notation "48"^^xsd:string;
  skos:prefLabel "Water Supply"@en ;
  skos:definition "Location where water supply can be"@en ;
  
   .

era-subloctype:50 a skos:Concept;
  skos:inScheme era-subloctype:SubsidiaryLocationTypes; 
  skos:topConceptOf era-subloctype:SubsidiaryLocationTypes ; 
  skos:note "Value collected from TAF/TAP -TSI code lists"@en;
  skos:notation "50"^^xsd:string;
  skos:prefLabel "Indoor cleaning platform"@en ;
  skos:definition "Place for interior cleaning"@en ;
  
   .

era-subloctype:51 a skos:Concept;
  skos:inScheme era-subloctype:SubsidiaryLocationTypes; 
  skos:topConceptOf era-subloctype:SubsidiaryLocationTypes ; 
  skos:note "Value collected from TAF/TAP -TSI code lists"@en;
  skos:notation "51"^^xsd:string;
  skos:prefLabel "Car-wash"@en ;
  skos:definition "Place for outdoor cleaning"@en ;
  
   .

era-subloctype:52 a skos:Concept;
  skos:inScheme era-subloctype:SubsidiaryLocationTypes; 
  skos:topConceptOf era-subloctype:SubsidiaryLocationTypes ; 
  skos:note "Value collected from TAF/TAP -TSI code lists"@en;
  skos:notation "52"^^xsd:string;
  skos:prefLabel "Short dry- cleaning track"@en ;
  skos:definition "Place for special cleaning"@en ;
  
   .

era-subloctype:54 a skos:Concept;
  skos:inScheme era-subloctype:SubsidiaryLocationTypes; 
  skos:topConceptOf era-subloctype:SubsidiaryLocationTypes ; 
  skos:note "Value collected from TAF/TAP -TSI code lists"@en;
  skos:notation "54"^^xsd:string;
  skos:prefLabel "Sand-filling station"@en ;
  skos:definition "Location where sand is filled."@en ;
  
   .

era-subloctype:56 a skos:Concept;
  skos:inScheme era-subloctype:SubsidiaryLocationTypes; 
  skos:topConceptOf era-subloctype:SubsidiaryLocationTypes ; 
  skos:note "Value collected from TAF/TAP -TSI code lists"@en;
  skos:notation "56"^^xsd:string;
  skos:prefLabel "Signal box"@en ;
  skos:definition "A building containing signalling equipment and staff."@en ;
  
   .

era-subloctype:57 a skos:Concept;
  skos:inScheme era-subloctype:SubsidiaryLocationTypes; 
  skos:topConceptOf era-subloctype:SubsidiaryLocationTypes ; 
  skos:note "Value collected from TAF/TAP -TSI code lists"@en;
  skos:notation "57"^^xsd:string;
  skos:prefLabel "Intermodal Terminal"@en ;
  skos:definition "Intermodal Terminal is a location which provides the space, equipment and operational environment under which the transfer of loading units (freight containers, swap bodies,"@en ;
  
   .

era-subloctype:58 a skos:Concept;
  skos:inScheme era-subloctype:SubsidiaryLocationTypes; 
  skos:topConceptOf era-subloctype:SubsidiaryLocationTypes ; 
  skos:note "Value collected from TAF/TAP -TSI code lists"@en;
  skos:notation "58"^^xsd:string;
  skos:prefLabel "OSJD system"@en ;
  skos:definition "Location code used within OSJD."@en ;
  
   .

era-subloctype:59 a skos:Concept;
  skos:inScheme era-subloctype:SubsidiaryLocationTypes; 
  skos:topConceptOf era-subloctype:SubsidiaryLocationTypes ; 
  skos:note "Value collected from TAF/TAP -TSI code lists"@en;
  skos:notation "59"^^xsd:string;
  skos:prefLabel "Train Service Substitute Stop"@en ;
  skos:definition "Place outside of railway station or railway stop, where passengers board or leave bus or any other transport mean as substitution of"@en ;
  
   .

era-subloctype:60 a skos:Concept;
  skos:inScheme era-subloctype:SubsidiaryLocationTypes; 
  skos:topConceptOf era-subloctype:SubsidiaryLocationTypes ; 
  skos:note "Value collected from TAF/TAP -TSI code lists"@en;
  skos:notation "60"^^xsd:string;
  skos:prefLabel "Multifunction al rail terminal"@en ;
  skos:definition "Facilities for conventional and/or intermodal rail/road transshipment principally open for public use and for all types of cargo. This kind of"@en ;
  
   .

era-subloctype:61 a skos:Concept;
  skos:inScheme era-subloctype:SubsidiaryLocationTypes; 
  skos:topConceptOf era-subloctype:SubsidiaryLocationTypes ; 
  skos:note "Value collected from TAF/TAP -TSI code lists"@en;
  skos:notation "61"^^xsd:string;
  skos:prefLabel "Relief facility"@en ;
  skos:definition "Facilities providing equipment and infrastructure used to overcome a disruption (derailment, collision or other accidents)."@en ;
  
   .


era-subloctype:70 a skos:Concept;
  skos:inScheme era-subloctype:SubsidiaryLocationTypes; 
  skos:topConceptOf era-subloctype:SubsidiaryLocationTypes ; 
  skos:note "Value collected from TAF/TAP -TSI code lists"@en;
  skos:notation "70"^^xsd:string;
  skos:prefLabel "Network Border"@en ;
  skos:definition "Network border between two neighboring IM's; first or last Primary Location on a network."@en ;
  skos:scopeNote "See details in Sector handbook"@en ;
  
   .


era-subloctype:71 a skos:Concept;
  skos:inScheme era-subloctype:SubsidiaryLocationTypes; 
  skos:topConceptOf era-subloctype:SubsidiaryLocationTypes ; 
  skos:note "Value collected from TAF/TAP -TSI code lists"@en;
  skos:notation "71"^^xsd:string;
  skos:prefLabel "State border"@en ;
  skos:definition "Political border between two"@en ;
  skos:scopeNote "See details in Sector"@en ;
  
   .

era-subloctype:72 a skos:Concept;
  skos:inScheme era-subloctype:SubsidiaryLocationTypes; 
  skos:topConceptOf era-subloctype:SubsidiaryLocationTypes ; 
  skos:note "Value collected from TAF/TAP -TSI code lists"@en;
  skos:notation "72"^^xsd:string;
  skos:prefLabel "Administrative border"@en ;
  skos:definition "Border point inside a member state to define federal structures or"@en ;
  skos:scopeNote "See details in Sector handbook"@en ;
  
   .


era-subloctype:74 a skos:Concept;
  skos:inScheme era-subloctype:SubsidiaryLocationTypes; 
  skos:topConceptOf era-subloctype:SubsidiaryLocationTypes ; 
  skos:note "Value collected from TAF/TAP -TSI code lists"@en;
  skos:notation "74"^^xsd:string;
  skos:prefLabel "Operational handover"@en ;
  skos:definition "Location where the responsibility for operation changes or can change between two involved IMs."@en ;
  skos:scopeNote "See details in Sector handbook"@en ;
  
   .

era-subloctype:75 a skos:Concept;
  skos:inScheme era-subloctype:SubsidiaryLocationTypes; 
  skos:topConceptOf era-subloctype:SubsidiaryLocationTypes ; 
  skos:note "Value collected from TAF/TAP -TSI code lists"@en;
  skos:notation "75"^^xsd:string;
  skos:prefLabel "Planning handover"@en ;
  skos:definition "Location where the responsibility for timetable planning and path allocation changes or can change between two involved IMs"@en ;
  skos:scopeNote "See details in Sector handbook Remark: \"Handover\" in this definition applies both for \"handover\" (entry in a network) and \"transfer\" (exit from a network) as currently used in xsd-elements: ScheduledTimeAtHand over and ScheduledDateTimeAtT ransfer"@en ;
  
   .


era-subloctype:76 a skos:Concept;
  skos:inScheme era-subloctype:SubsidiaryLocationTypes; 
  skos:topConceptOf era-subloctype:SubsidiaryLocationTypes ; 
  skos:note "Value collected from TAF/TAP -TSI code lists"@en;
  skos:notation "76"^^xsd:string;
  skos:prefLabel "Stopping"@en ;
  skos:definition "This SLC defines a point along a track"@en ;
  skos:scopeNote """New code 
                              TAF messages: Train running messages,
                              Train running forecast (priority),
                              Change of track, Path details"""@en ;
  
   .


era-subloctype:99 a skos:Concept;
  skos:inScheme era-subloctype:SubsidiaryLocationTypes; 
  skos:topConceptOf era-subloctype:SubsidiaryLocationTypes ; 
  skos:note "Value collected from TAF/TAP -TSI code lists"@en;
  skos:notation "99"^^xsd:string;
  skos:prefLabel "Relation to Station"@en ;
  skos:definition "An indicator used to show that this location is a subsidiary of another"@en ;
  
   .





