@prefix rdf: <http://www.w3.org/1999/02/22-rdf-syntax-ns#> .
@prefix rdfs: <http://www.w3.org/2000/01/rdf-schema#> .
@prefix owl: <http://www.w3.org/2002/07/owl#> .
@prefix xsd: <http://www.w3.org/2001/XMLSchema#> .
@prefix dcterms: <http://purl.org/dc/terms/> .
@prefix skos: <http://www.w3.org/2004/02/skos/core#> .
@prefix cc: <http://creativecommons.org/ns#> .
@prefix era: <http://data.europa.eu/949/> .
@prefix era-skos: <http://data.europa.eu/949/concepts/> .
@prefix era-va-authcase: <http://data.europa.eu/949/concepts/va-authcases/> .



#################################################################
#
#    Concept Schemes
#
#################################################################
era-va-authcase:VehicleAuthorisationCase a skos:ConceptScheme ;
    dcterms:issued "2024-05-22"^^xsd:date ;
    cc:license <https://creativecommons.org/licenses/by/4.0/> ;
    rdfs:comment "Controlled SKOS-based vocabularies defined by the European Union Agency for Railways (see https://www.era.europa.eu/domains/applicants/applications-vehicle-type-authorisations_en)."@en ;
    rdfs:label "Identification of the relevant authorisation cases (Art.14)"@en ;
    dcterms:title "Concept scheme grouping the vehicle authorisation cases"@en .



#################################################################
#
#    Concept instances
#
#################################################################



########## Vehicle authorisation cases ##########

era-va-authcase:FA a skos:Concept ;
    skos:topConceptOf era-va-authcase:VehicleAuthorisationCase ;
    skos:inScheme era-va-authcase:VehicleAuthorisationCase ; 
    skos:definition "The vehicle type authorisation and/or the vehicle authorisation for placing on the market issued by the authorising entity for a new vehicle type, including its variants and/or versions if any, and, where applicable, the first vehicle of a type, pursuant to Article 21(1) of Directive (EU) 2016/797."@en ;
    skos:prefLabel "First Authorisation"@en ;
    dcterms:source <http://data.europa.eu/eli/reg_impl/2018/545/oj> .
    

era-va-authcase:RENEW a skos:Concept ;
    skos:topConceptOf era-va-authcase:VehicleAuthorisationCase ;
    skos:inScheme era-va-authcase:VehicleAuthorisationCase ; 
    skos:definition "The renewal of a vehicle type authorisation pursuant to Article 24(3) of Directive (EU) 2016/797 which does not require a change in design of the vehicle type."@en ;
    skos:prefLabel "Renewed vehicle type authorisation"@en ;
   dcterms:source <http://data.europa.eu/eli/reg_impl/2018/545/oj> .

era-va-authcase:EXT a skos:Concept ;
    skos:topConceptOf era-va-authcase:VehicleAuthorisationCase ;
    skos:inScheme era-va-authcase:VehicleAuthorisationCase ;
    skos:definition "The vehicle type authorisation and/or the vehicle authorisation for placing on the market issued by the relevant authorising entity for an already authorised vehicle type and/or vehicle in order to extend the area of use without a change of the design, pursuant to Article 21(13) of Directive (EU) 2016/797."@en ;
    skos:prefLabel "Extended area of use"@en ;
    dcterms:source <http://data.europa.eu/eli/reg_impl/2018/545/oj> .

era-va-authcase:NEW a skos:Concept ;
    skos:topConceptOf era-va-authcase:VehicleAuthorisationCase ;
    skos:inScheme era-va-authcase:VehicleAuthorisationCase ; 
    skos:definition "The vehicle type authorisation and/or vehicle authorisation for placing on the market issued by the authorising entity after a change of an already authorised vehicle and/or vehicle type, pursuant to Articles 21(12) or 24(3) of Directive (EU) 2016/797."@en ;
    skos:prefLabel "New Authorisation"@en ;
   dcterms:source <http://data.europa.eu/eli/reg_impl/2018/545/oj> .

era-va-authcase:C2T a skos:Concept ;
    skos:topConceptOf era-va-authcase:VehicleAuthorisationCase ;
    skos:inScheme era-va-authcase:VehicleAuthorisationCase ; 
    skos:definition "The vehicle authorisation for placing on the market for a vehicle or a series of vehicles that conform to an already authorised and valid vehicle type on the basis of a declaration of conformity to that type, pursuant to Article 25(1) of Directive (EU) 2016/797. Where applicable, there shall be a clear identification of the vehicle type version and/or the vehicle type variant to which the vehicle or series of vehicles is conform."@en ;
    skos:prefLabel "Authorisation in conformity to type"@en ;
    dcterms:source <http://data.europa.eu/eli/reg_impl/2018/545/oj> .
